fix proof; bring LocV back

src/examples/implang_cont_eg.v
@@ -8,12 +8,12 @@ Local Open Scope func_scope.
 Definition min_positive :=
   fn "l" <{ ( "min" "v" )
     "min" <a- #0 ;;
-    While "l" ≠ #0 <{
-      (* If !"l" < !"min" <{ break }> ;; *)
+    While #1 <{
+      If "l" = #0 <{ break }> ;;
       "v" <a- !"l";;
       "l" <a- !("l" + #1);;
       If "v" <= #0 <{ continue }> ;;
-      If "min" = #0 || "v" < "min" <{ "min" <a- "v" }> 
+      If ("min" = #0) || ("v" < "min") <{ "min" <a- "v" }>
     }>;;
     Return "min"
   }>.
@@ -28,24 +28,125 @@ Section spec.
   Local Open Scope bi_scope.
   Local Open Scope Z_scope.
 
-  Definition min_positive_r (lv: list Z) : Z :=
-    Z.max 0 (foldr Z.min 0 lv).
+  Definition pos_elems (l: list Z) :=
+    filter (λ x, x > 0) l.
 
-  Lemma min_positive_r_cons x l : min_positive_r (x::l) = Z.max 0 (Z.min x (min_positive_r l)).
+  Definition min_l (l: list Z) : Z :=
+    match l with
+    | [] => 0
+    | h::t => foldr Z.min h t
+    end.
+
+  Definition min_positive_r (n: Z) (l: list Z) : Prop :=
+    let l' := pos_elems l in
+    ((n = 0 ∧ l' = []) ∨ n=min_l l').
+
+  Definition compute_min_positive (l: list Z) : Z :=
+    min_l (pos_elems l).
+
+  Lemma compute_min_positive_is_min_positive_r l :
+    min_positive_r (compute_min_positive l) l.
   Proof.
-    rewrite /min_positive_r /=. lia.
+     rewrite /compute_min_positive /min_positive_r.
+     right. done.
+  Qed.
+  
+  Lemma min_l_cons x l :
+    l ≠ [] ->
+    min_l (x::l) = Z.min x (min_l l).
+  Proof.
+    intros. destruct l; try done.
+    simpl.
+    rewrite -!foldr_comm_acc.
+    2-3: intros; rewrite !Z.min_assoc [X in Z.min X _]Z.min_comm //.
+    rewrite [X in foldr _ X _]Z.min_comm //.
   Qed.
 
-  Lemma min_positive_r_app_r (lv_a : list Z) (z: Z) :
-    z ≤ 0 →
-    min_positive_r (lv_a ++ [z]) = min_positive_r lv_a.
+  Lemma pos_elems_cons x l :
+    pos_elems (x::l) = (if bool_decide (x > 0) then [x] else []) ++ pos_elems l.
   Proof.
-    revert z.
+    intros. rewrite /pos_elems filter_cons decide_bool_decide //.
+    destruct (bool_decide (x > 0)) eqn:Heq; done.
+  Qed.
+
+  Lemma foldr_Z_min_in_list h t :
+     foldr Z.min h t ∈ h::t.
+  Proof.
+    induction t; simpl; try done.
+    - constructor.
+    - destruct (Z.min_dec a (foldr Z.min h t)).
+      + rewrite e. repeat constructor.
+      + rewrite e. eapply elem_of_subseteq. 2: apply IHt.
+        intros.
+        rewrite /elem_of in H.
+        inversion H; subst; by repeat constructor.
+  Qed.
+
+
+  Lemma pos_elems_foldr_ge_0 l h t:
+    pos_elems l = h :: t -> foldr Z.min h t > 0.
+  Proof.
+    intros.
+    set (foldr Z.min h t) as m.
+    assert (m ∈ pos_elems l). { rewrite H. apply foldr_Z_min_in_list. }
+    rewrite elem_of_list_filter in H0. easy.
+  Qed.
+
+  Lemma compute_min_positive_cons x l :
+    compute_min_positive (x::l) = if bool_decide (x > 0 ∧ (compute_min_positive l = 0 ∨ x < compute_min_positive l)) 
+                                  then x else compute_min_positive l.
+  Proof.
+    intros.
+    rewrite {1}/compute_min_positive pos_elems_cons /=.
+    destruct (bool_decide (x > 0)) eqn:Heqx.
+    2: { rewrite bool_decide_and Heqx //. }
+    destruct (pos_elems l) eqn:Hpos.
+    { rewrite /compute_min_positive Hpos /=. rewrite bool_decide_and Heqx //. }
+    rewrite min_l_cons //. rewrite -Hpos.
+    rewrite bool_decide_and Heqx /=. 
+    assert (bool_decide (compute_min_positive l = 0) = false).
+    {
+      apply bool_decide_eq_false. rewrite /compute_min_positive /=.
+      apply pos_elems_foldr_ge_0 in Hpos as ?.
+      rewrite /min_l Hpos.
+      lia.
+     }
+    rewrite bool_decide_or H /=.
+    destruct (bool_decide (x < compute_min_positive l)) eqn:Heq2.
+    - rewrite bool_decide_eq_true /compute_min_positive in Heq2.
+      lia.
+    - rewrite bool_decide_eq_false /compute_min_positive in Heq2.
+      rewrite /compute_min_positive. lia.
+  Qed.
+
+  Lemma compute_min_positive_snoc x l : compute_min_positive (l++[x]) = compute_min_positive ([x]++l).
+  Proof.
+     revert x.
+     induction l; intros.
+    - rewrite /compute_min_positive /min_l /pos_elems /=.
+      destruct (decide (x > 0)) eqn:Heq; try lia.
+    - rewrite -app_comm_cons !compute_min_positive_cons !IHl.
+  Admitted.
+
+  Lemma compute_min_positive_app_comm (lv_a lv_b: list Z) :
+    compute_min_positive (lv_a ++ lv_b) = compute_min_positive (lv_b ++ lv_a).
+  Proof.
+    revert lv_b.
     induction lv_a as [|x lv_a IH]; intros.
-    - rewrite /min_positive_r /=; lia.
-    - rewrite -app_comm_cons min_positive_r_cons IH //.
-      rewrite /min_positive_r /=. lia.
+    - rewrite app_nil_r app_nil_l //.
+    - rewrite -app_comm_cons cons_middle app_assoc -IH app_assoc
+      compute_min_positive_snoc //.
   Qed.
+
+  Lemma min_positive_r_app (lv_a : list Z) (z: Z) :
+    z ≤ 0 →
+    compute_min_positive (lv_a ++ [z]) = compute_min_positive lv_a.
+  Proof.
+    rewrite compute_min_positive_snoc compute_min_positive_cons => ?.
+    rewrite bool_decide_and.
+    destruct (bool_decide (z > 0)) eqn:Hz; [rewrite bool_decide_eq_true in Hz; lia|].
+    done.
+  Qed. 
 
   Definition ptr_add (l: loc) (i: Z) : loc :=
     (l + i)%Z.
@@ -53,13 +154,13 @@ Section spec.
 
   (* a segment of linked list starting with l and stores lv;
     the last cell has pointer `last` that might or might not be empty *)
-  Fixpoint llist_seg (l: loc) (lv: list Z) (last: loc) : assert :=
+  Fixpoint llist_seg (l: val) (lv: list Z) (last: val) : assert :=
     match lv with
     | [] => ⌜l = last⌝
-    | v :: lv' => ⌜l≠0%Z⌝ ∧ ∃ l', l ↦ NumV v ∗ (l+ₗ1) ↦ LocV l' ∗ llist_seg l' lv' last
+    | v :: lv' => ∃ p, ⌜l=LocV p⌝ ∧ ∃ l', p ↦ NumV v ∗ (p+ₗ1) ↦ l' ∗ llist_seg l' lv' last
     end.
 
-  Definition llist (l: loc) (lv: list Z) := llist_seg l lv 0%Z.
+  Definition llist (l: val) (lv: list Z) := llist_seg l lv 0.
 
   Global Instance llist_seg_objective l lv last : Objective (llist_seg l lv last).
   Proof.
@@ -82,9 +183,9 @@ Section spec.
     induction lv1 => ?; simpl.
     - iSplit; by [iIntros "$"|iIntros "(% & -> & $)"].
     - iSplit; iIntros "H".
-      + iDestruct "H" as "(% & %l' & $ & $ & H3)". rewrite IHlv1.
+      + iDestruct "H" as "(%l' & % & % & $ & $ & H3)". rewrite IHlv1.
         by iDestruct "H3" as "(% & $ & $)".
-      + iDestruct "H" as "(% & (% & % & $ & $ & H2) & H3)".
+      + iDestruct "H" as "(% & (%& % & % & $ & $ & H2) & H3)".
         iSplit; first done. rewrite IHlv1. iFrame.
   Qed.
 
@@ -99,9 +200,9 @@ Section spec.
   (* ad-hoc, aggressive *)
   Ltac iSteps := repeat first [iStep | iModIntro | progress iFrame | progress iIntros | progress simpl].
 
-  Lemma min_positive_spec E (l: loc) (lv: list Z) :
+  Lemma min_positive_spec E (l: val) (lv: list Z) :
     (∃ _z, "r" ↦v NumV _z) ∗ l ↦ₗ lv
-    ⊢ call_assert F E min_positive [LocV l; NumV 0; NumV 0] "r" ("r" ↦v NumV (min_positive_r lv) ∗ l ↦ₗ lv).
+    ⊢ call_assert F E min_positive [l; NumV 0; NumV 0] "r" (∃ r, ⌜min_positive_r r lv⌝ ∧ "r" ↦v NumV r ∗ l ↦ₗ lv).
   Proof.
     iIntros "((%_z & r) & arr)".
     wp_start_func with_retainer "retainer" and_locals "(l & min & v & _)".
@@ -110,42 +211,91 @@ Section spec.
           (* split arr into two parts *)
           ⌜lv = lv_a++lv_b ⌝ ∧ l ↦ₛ lv_a l_m ∗ l_m ↦ₗ lv_b ∗ 
           (* "min" always store min of the first part*)
-          "l" ↦v (LocV l_m) ∗ "v" ↦v v ∗ "min" ↦v (NumV (min_positive_r lv_a)) ∗
+          "l" ↦v l_m ∗ "v" ↦v v ∗ "min" ↦v (NumV (compute_min_positive lv_a)) ∗
           stack_retainer min_positive ∗ (∃ _z, ⇓ ("r" ↦v _z)))%I%Z as inv.
     wp_apply (wp_while_inv  _ _ _ _ inv with "[] [-]" ); simpl.
     {
       iIntros "!> (%l_m & %lv_a & %lv_b & %v & -> & arr_a & arr_b & l & v & min & retainer & (%_z' & r))".
       iSteps.
-      destruct (bool_decide (l_m = 0%Z)) eqn: Heqb; rewrite Heqb;
+      iExists _. iSplit; first done.
+      iSteps.
+      destruct (bool_decide (l_m = 0)) eqn: Heqb;
         [rewrite bool_decide_eq_true in Heqb; subst | rewrite bool_decide_eq_false in Heqb].
       - iExists _. iSplit; first done.
         iSteps.
         iSplitL "l v min".
         { iExists [_;_;_]. iSplit; first done. by iFrame. }
         iIntros "!> !> r". iFrame.
-        destruct lv_b. 2: { iDestruct "arr_b" as "[% ?]". done. }
-        rewrite app_nil_r. iFrame.
-      - iExists _. iSplit; first done.
+        destruct lv_b. 2: { iDestruct "arr_b" as "(% & % & % & ?)". done. }
+        rewrite app_nil_r. iFrame. iPureIntro. apply compute_min_positive_is_min_positive_r.
+      - simpl.
+        destruct (lv_b).
+        { iDestruct "arr_b" as "->". simpl.
+          iExists _. iSplit; first done.
+          iSteps.
+          iSplitL "l v min".
+          { iExists [_]. iSplit; first done. by iFrame. }
+          iIntros "!> !> r". iFrame.
+          rewrite app_nil_r. by iFrame.
+        }
+
+        iDestruct "arr_b" as "(% & -> & %l' & arr_b_0 & arr_b_1 & arr_c)".
+        fold llist_seg.
+        simpl.
+        iExists _. iSplit; first done.
         iSteps.
-        destruct lv_b. { iDestruct "arr_b" as "%". done. }
-        iDestruct "arr_b" as "(% & %l_n & arr_b_0 & arr_b_1 & arr_c)". fold llist_seg.
-        iFrame. iIntros "arr_b_0".
-        iFrame. iIntros "!> v".
+        iExists _. iSplit; first done.
         iSteps.
-        destruct (bool_decide (z ≤ 0)%Z) eqn:Heqz;
-          [rewrite bool_decide_eq_true in Heqz; subst | rewrite bool_decide_eq_false in Heqz].
-        + iExists _. iSplit; first done.
-          iModIntro. simpl. iStep. simpl.
-          iRename select (⎡pointsto (l_m + 1)%Z _ _⎤)%I into "arr_b_1".
-          iPoseProof (bi.equiv_entails_1_2  _ _ (llist_seg_app l lv_a [z] l_n) with "[$arr_a $arr_b_0 $arr_b_1]") as "?".
+        destruct (bool_decide (z ≤ 0)%Z) eqn:Heqz.
+        +  simpl. iStep. simpl.
+          iRename select (⎡pointsto _ _ l'⎤) into "arr_b_1".
+          iRename select (⎡pointsto _ _ (NumV z)⎤) into "arr_b_0".
+          iPoseProof (bi.equiv_entails_1_2  _ _ (llist_seg_app l lv_a [z] _) with "[$arr_a $arr_b_0 $arr_b_1]") as "?".
           { done. }
           iFrame.
-          rewrite -app_assoc /= min_positive_r_app_r //.
-          by iFrame.
-        + iExists _. iSplit; first done.
+          rewrite -app_assoc min_positive_r_app //=. by iFrame. rewrite bool_decide_eq_true // in Heqz.
+        + destruct (bool_decide (z > 0)) eqn: Heqz'.
+          2: { rewrite bool_decide_eq_false in Heqz'.
+                rewrite bool_decide_eq_false  in Heqz.
+                lia. }
           iSteps.
-          (* FIXME fill in the boring case analysis here *)
-          admit.
+          iExists _. iSplit; first done.
+          iSteps.
+          destruct (bool_decide ((compute_min_positive lv_a = 0) ∨ (z < compute_min_positive lv_a))) eqn:Heq1;
+          rewrite bool_decide_or in Heq1.
+          ++ rewrite orb_true_iff in Heq1.
+            destruct Heq1 as [Heq1 | Heq1]; simpl.
+            +++ rewrite Heq1. iSteps. rewrite {1}cons_middle {1}app_assoc. iExists _; iSplit; first done.
+                rewrite llist_seg_app. iFrame.
+                rewrite compute_min_positive_snoc compute_min_positive_cons.
+                rewrite bool_decide_and bool_decide_or Heq1 Heqz' /=.
+                by iFrame.
+            +++ rewrite !Heq1.
+                assert (bool_decide (compute_min_positive lv_a = 0) = false) as ?.
+                {
+                  rewrite bool_decide_eq_true in Heq1.
+                  rewrite bool_decide_eq_false in Heqz.
+                  apply bool_decide_eq_false. lia. 
+                }
+                rewrite H /=.
+                iSteps.
+                rewrite {1}cons_middle {1}app_assoc. iExists _; iSplit; first done.
+                rewrite llist_seg_app. iFrame.
+                iSplit; first done.
+                rewrite compute_min_positive_snoc compute_min_positive_cons bool_decide_and bool_decide_or.
+                rewrite Heqz' H Heq1 //.
+          ++ rewrite orb_false_iff in Heq1.
+            destruct Heq1 as [Heq1  Heq2].
+            rewrite Heq1 Heq2 /=.
+            iStep. simpl.
+            rewrite /inv.
+            rewrite {1}cons_middle {1}app_assoc.
+            iExists _, _, _, _. iSplit; first done.
+            iFrame.
+            rewrite llist_seg_app. iFrame.
+            iSplit; first done.
+            rewrite compute_min_positive_snoc compute_min_positive_cons bool_decide_and bool_decide_or.
+            rewrite Heqz' Heq1 Heq2 //.
     }
     {
       rewrite /inv. iFrame. iExists []. rewrite app_nil_l /=. by iFrame.
@@ -154,15 +304,16 @@ Section spec.
     iRename select (_) into "inv".
     iDestruct "inv" as "(%l_m & %lv_a & %lv_b & %v & -> & arr_a & arr_b & l & v & min & retainer & (%_z' & r))".
     iSteps.
-    rewrite /BoolV in H.
-    destruct (bool_decide (l_m = 0%Z)) eqn:Heqb; rewrite Heqb in H;
-      [rewrite bool_decide_eq_true in Heqb; subst | done].
+    (* destruct (bool_decide (l_m = 0%Z)) eqn:Heqb; rewrite Heqb in H;
+      [rewrite bool_decide_eq_true in Heqb; subst | done]. *)
     iSplitL "l v min".
     { iExists [_;_;_]. iSplit; first done. by iFrame. }
     iIntros "!> !> r". iFrame.
     destruct lv_b. 2: { rewrite /llist {2}/llist_seg /=. iDestruct "arr_b" as "[% ?]". done. }
-    rewrite app_nil_r. iFrame.
-  Admitted.
+    rewrite app_nil_r.
+    iDestruct "arr_b" as "->". iFrame.
+    iPureIntro. apply compute_min_positive_is_min_positive_r.
+  Qed.
 
 End spec.
 
